[SEM_CHNG] Sanitize semantics of select

src/Vellvm/opsem.v
@@ -488,6 +488,14 @@ match (getOperandValue TD v1 lc gl, getOperandValue TD v2 lc gl) with
 end
 .
 
+Definition SELECT (TD:TargetData) (lc gl:GVMap) (v0 v1 v2:value) (t: typ): option GenericValue :=
+  match (getOperandValue TD v0 lc gl, getOperandValue TD v1 lc gl, getOperandValue TD v2 lc gl) with
+  | (Some gv0, Some gv1, Some gv2) => mselect TD t gv0 gv1 gv2
+  | _ => None (* gundef TD t *)
+           (* for unity *)
+  end
+.
+
 Definition CAST (TD:TargetData) (lc:GVsMap) (gl:GVMap) (op:castop)
   (t1:typ) (v1:value) (t2:typ) : option GenericValue:=
 match (getOperandValue TD v1 lc gl) with
@@ -554,18 +562,6 @@ Proof.
   unfold isGVZero. rewrite INT.
   destruct (zeq z 0); simpl in DECISION; rewrite DECISION; auto.
 Qed.
-
-Inductive calc_select (TD:TargetData) (t:typ) (gv gvs1 gvs2 gvresult:GenericValue) : Prop :=
-| select_cond_def
-    z
-    (INT: GV2int TD Size.One gv = Some z)
-    (RESULT: gvresult = if (negb (zeq z 0)) then gvs1 else gvs2)
-| select_cond_undef
-    gvundef
-    (NOINT: GV2int TD Size.One gv = None)
-    (UNDEF: gundef TD t = Some gvundef)
-    (RESULT: gvresult = gvundef)
-.
 
 Definition intConst2Z c :=
   match c with
@@ -844,12 +840,8 @@ Inductive sInsn : Config -> State -> State -> trace -> Prop :=
     (mkState (mkEC F B cs tmn (updateAddAL _ lc id gvs3) als) (ECS) Mem)
     E0
 
-| sSelect : forall S TD Ps F B lc gl fs id v0 t v1 v2 c ECS cs tmn Mem als
-                    gvs1 gvs2 gvresult,
-  getOperandValue TD v0 lc gl = Some c ->
-  getOperandValue TD v1 lc gl = Some gvs1 ->
-  getOperandValue TD v2 lc gl = Some gvs2 ->
-  calc_select TD t c gvs1 gvs2 gvresult ->
+| sSelect : forall S TD Ps F B lc gl fs id v0 t v1 v2 ECS cs tmn Mem als gvresult,
+    SELECT TD lc gl v0 v1 v2 t = Some gvresult ->
   sInsn (mkCfg S TD Ps gl fs)
     (mkState (mkEC F B ((insn_select id v0 t v1 v2)::cs) tmn lc als) (ECS) Mem)
     (mkState (mkEC F B cs tmn (updateAddAL _ lc id gvresult) als) (ECS) Mem)
